Here is the rendered LaTeX:

---

Alright, let's tackle this problem step by step. I'm trying to prove that the implication \( p \rightarrow (q \land r) \) is logically equivalent to \( (\neg q \land \neg r) \rightarrow \neg p \) using resolution. 

### Understanding the Problem

First, let's recall what logical equivalence means. Two statements are logically equivalent if they have the same truth value in all possible scenarios. The resolution is a method used in automated theorem proving, which involves refuting the negation of the statement we want to prove to show that the original statement is valid.

Given two implications:
1. \( p \rightarrow (q \land r) \)
2. \( (\neg q \land \neg r) \rightarrow \neg p \)

We need to show that these are equivalent using resolution.

### Step 1: Convert Implications to Disjunctions

First, let's recall that an implication \( A \rightarrow B \) can be rewritten as \( \neg A \lor B \).

So, let's rewrite both implications:

1. \( p \rightarrow (q \land r) \) becomes \( \neg p \lor (q \land r) \).
2. \( (\neg q \land \neg r) \rightarrow \neg p \) becomes \( \neg (\neg q \land \neg r) \lor \neg p \).

Simplifying the second one:
\( \neg (\neg q \land \neg r) \) is \( q \lor r \) (by De Morgan's laws), so it becomes \( (q \lor r) \lor \neg p \), which is the same as \( q \lor r \lor \neg p \) (associativity of disjunction).

So now we have:
1. \( \neg p \lor (q \land r) \)
2. \( \neg p \lor q \lor r \)

Hmm, these don't look the same yet. Maybe there's a better approach.

### Step 2: Prove Equivalence by Showing Both Directions

To show that two statements are equivalent, we can show that each implies the other. That is:
- Show \( p \rightarrow (q \land r) \) implies \( (\neg q \land \neg r) \rightarrow \neg p \).
- Show \( (\neg q \land \neg r) \rightarrow \neg p \) implies \( p \rightarrow (q \land r) \).

Let's do this using resolution.

#### Direction 1: \( p \rightarrow (q \land r) \) implies \( (\neg q \land \neg r) \rightarrow \neg p \)

To show implication via resolution, we assume the negation of the consequent and try to derive a contradiction from the antecedent.

Assume:
1. \( p \rightarrow (q \land r) \) (given), which is \( \neg p \lor (q \land r) \).
2. Negation of \( (\neg q \land \neg r) \rightarrow \neg p \), which is \( \neg [ (\neg q \land \neg r) \rightarrow \neg p ] \).

The negation of \( A \rightarrow B \) is \( A \land \neg B \), so:
\( \neg q \land \neg r \land \neg \neg p \) which is \( \neg q \land \neg r \land p \).

Now, let's express these in CNF (Conjunctive Normal Form) for resolution:

From the given \( \neg p \lor (q \land r) \), we can distribute to get CNF:
\( (\neg p \lor q) \land (\neg p \lor r) \).

From the assumption (negation of the consequent):
\( \neg q \), \( \neg r \), \( p \).

Now, let's list all clauses:
1. \( \neg p \lor q \)
2. \( \neg p \lor r \)
3. \( \neg q \)
4. \( \neg r \)
5. \( p \)

Now, apply resolution:

- Resolve clause 1 (\( \neg p \lor q \)) with clause 3 (\( \neg q \)):
  \( \neg p \lor q \) and \( \neg q \) resolve to \( \neg p \).

- Now we have \( \neg p \) (from above) and \( p \) (clause 5):
  \( \neg p \) and \( p \) resolve to the empty clause (contradiction).

Since we've derived a contradiction from assuming the negation of the consequent, the original implication must hold.

#### Direction 2: \( (\neg q \land \neg r) \rightarrow \neg p \) implies \( p \rightarrow (q \land r) \)

Now, let's prove the other direction.

Given:
\( (\neg q \land \neg r) \rightarrow \neg p \), which is \( q \lor r \lor \neg p \).

We want to show \( p \rightarrow (q \land r) \), which is \( \neg p \lor (q \land r) \).

Assume the negation of \( p \rightarrow (q \land r) \):
\( \neg [ \neg p \lor (q \land r) ] \) which is \( p \land \neg (q \land r) \), i.e., \( p \land (\neg q \lor \neg r) \).

In CNF:
- \( p \)
- \( \neg q \lor \neg r \)

Given clauses:
1. \( q \lor r \lor \neg p \) (from the given implication)
2. \( p \) (from assumption)
3. \( \neg q \lor \neg r \) (from assumption)

Now, apply resolution:

- From clause 1 (\( q \lor r \lor \neg p \)) and clause 2 (\( p \)):
  \( \neg p \) in clause 1 is negated by \( p \), so we get \( q \lor r \).

Now we have:
- \( q \lor r \)
- \( \neg q \lor \neg r \)

Resolve \( q \lor r \) with \( \neg q \lor \neg r \):

Possible resolutions:
- \( q \) with \( \neg q \): gives \( r \lor \neg r \), which is always true (tautology, doesn't help).
- \( r \) with \( \neg r \): gives \( q \lor \neg q \), always true.

Hmm, this isn't leading to a contradiction directly. Maybe another approach.

Alternatively, let's consider that \( q \lor r \) and \( \neg q \lor \neg r \) together imply that one of \( q \) or \( r \) is true, and one is false. This doesn't directly contradict anything, which suggests that our approach might be missing something.

Wait, perhaps we need to consider that from \( q \lor r \) and \( \neg q \lor \neg r \), we can derive that exactly one of \( q \) or \( r \) is true, but this doesn't contradict our assumptions. Maybe we need to find another path.

Alternatively, let's recall that \( q \lor r \) and \( \neg q \lor \neg r \) imply \( (q \land \neg r) \lor (\neg q \land r) \), which is the XOR of \( q \) and \( r \). But this doesn't directly help in deriving a contradiction from our given clauses.

Perhaps the initial approach needs adjustment. Maybe instead of trying to derive a contradiction, we can show that the two forms are equivalent by transforming one into the other.

### Step 3: Alternative Approach - Transform One Side to the Other

Let's start with \( p \rightarrow (q \land r) \):
\( \neg p \lor (q \land r) \).

Distribute \( \lor \) over \( \land \):
\( (\neg p \lor q) \land (\neg p \lor r) \).

Now, let's look at \( (\neg q \land \neg r) \rightarrow \neg p \):
\( \neg (\neg q \land \neg r) \lor \neg p \)
\( (q \lor r) \lor \neg p \)
\( q \lor r \lor \neg p \).

Now, can we show that \( (\neg p \lor q) \land (\neg p \lor r) \) is equivalent to \( q \lor r \lor \neg p \)?

Actually, no, because the first is stronger (implies the second, but not vice versa). Wait, that can't be right because we're supposed to prove equivalence.

Wait, perhaps the initial interpretation is off. Maybe the equivalence is not directly between these two CNFs but through the implications.

Alternatively, let's consider that \( A \rightarrow B \) is equivalent to \( \neg B \rightarrow \neg A \). This is the contrapositive, and they are equivalent.

Given \( p \rightarrow (q \land r) \), its contrapositive is \( \neg (q \land r) \rightarrow \neg p \), which is \( (\neg q \lor \neg r) \rightarrow \neg p \).

But the right side of the original equation is \( (\neg q \land \neg r) \rightarrow \neg p \), which is different from \( (\neg q \lor \neg r) \rightarrow \neg p \).

Ah! So the original statement seems incorrect because the correct contrapositive of \( p \rightarrow (q \land r) \) is \( \neg (q \land r) \rightarrow \neg p \), which is \( (\neg q \lor \neg r) \rightarrow \neg p \), not \( (\neg q \land \neg r) \rightarrow \neg p \).

Therefore, the original equation \( p \rightarrow (q \land r) = (\neg q \land \neg r) \rightarrow \neg p \) is not correct because the right side should have \( \lor \) instead of \( \land \).

### Verifying with Truth Tables

To confirm, let's construct truth tables for both statements.

**Statement 1:** \( p \rightarrow (q \land r) \)

| p | q | r | q ∧ r | p → (q ∧ r) |
|---|---|---|-------|-------------|
| T | T | T |   T   |      T      |
| T | T | F |   F   |      F      |
| T | F | T |   F   |      F      |
| T | F | F |   F   |      F      |
| F | T | T |   T   |      T      |
| F | T | F |   F   |      T      |
| F | F | T |   F   |      T      |
| F | F | F |   F   |      T      |

**Statement 2:** \( (\neg q \land \neg r) \rightarrow \neg p \)

First, compute \( \neg q \land \neg r \), then \( \neg p \), then the implication.

| p | q | r | ¬q | ¬r | ¬q ∧ ¬r | ¬p | (¬q ∧ ¬r) → ¬p |
|---|---|---|----|----|--------|----|----------------|
| T | T | T | F  | F  |   F    | F  |       T        |
| T | T | F | F  | T  |   F    | F  |       T        |
| T | F | T | T  | F  |   F    | F  |       T        |
| T | F | F | T  | T  |   T    | F  |       F        |
| F | T | T | F  | F  |   F    | T  |       T        |
| F | T | F | F  | T  |   F    | T  |       T        |
| F | F | T | T  | F  |   F    | T  |       T        |
| F | F | F | T  | T  |   T    | T  |       T        |

Now, compare the last columns:

For \( p \rightarrow (q \land r) \): T, F, F, F, T, T, T, T  
For \( (\neg q \land \neg r) \rightarrow \neg p \): T, T, T, F, T, T, T, T  

They differ in the second and third rows where \( p \) is true, \( q \) and \( r \) are not both false, but one is false. For example, when \( p=T, q=T, r=F \):
- \( p \rightarrow (q \land r) = F \)
- \( (\neg q \land \neg r) \rightarrow \neg p = T \) (since \( \neg q \land \neg r = F \), and \( F \rightarrow F = T \))

Thus, the two statements are not equivalent.

### Conclusion

After carefully working through the problem, it appears that the original statement claiming that \( p \rightarrow (q \land r) \) is equivalent to \( (\neg q \land \neg r) \rightarrow \neg p \) is incorrect. The correct contrapositive of \( p \rightarrow (q \land r) \) is \( \neg (q \land r) \rightarrow \neg p \), which is \( (\neg q \lor \neg r) \rightarrow \neg p \), not \( (\neg q \land \neg r) \rightarrow \neg p \). The truth tables also confirm that these two expressions are not equivalent.

Therefore, the given equivalence does not hold. There might be a typo in the original problem where \( \land \) should be \( \lor \) in the second part. The correct equivalence is:

$$ p \rightarrow (q \land r) \equiv (\neg q \lor \neg r) \rightarrow \neg p $$

### Correct Proof of the Correct Equivalence

For completeness, let's prove the correct equivalence using resolution.

**Prove:** \( p \rightarrow (q \land r) \equiv (\neg q \lor \neg r) \rightarrow \neg p \)

We'll show both directions.

#### Direction 1: \( p \rightarrow (q \land r) \) implies \( (\neg q \lor \neg r) \rightarrow \neg p \)

Given: \( \neg p \lor (q \land r) \), which is \( (\neg p \lor q) \land (\neg p \lor r) \).

Negation of consequent: \( \neg [ (\neg q \lor \neg r) \rightarrow \neg p ] \), which is \( (\neg q \lor \neg r) \land p \).

Clauses:
1. \( \neg p \lor q \)
2. \( \neg p \lor r \)
3. \( \neg q \lor \neg r \)
4. \( p \)

Resolution:
- Resolve 1 and 4: \( \neg p \lor q \) with \( p \) gives \( q \).
- Resolve 2 and 4: \( \neg p \lor r \) with \( p \) gives \( r \).
Now have \( q \) and \( r \).
- Resolve \( q \) with \( \neg q \lor \neg r \): choose \( q \) and \( \neg q \) to get \( \neg r \).
Now have \( r \) and \( \neg r \), which resolve to empty clause (contradiction).

#### Direction 2: \( (\neg q \lor \neg r) \rightarrow \neg p \) implies \( p \rightarrow (q \land r) \)

Given: \( \neg (\neg q \lor \neg r) \lor \neg p \), which is \( (q \land r) \lor \neg p \), same as \( \neg p \lor (q \land r) \).

This is exactly \( p \rightarrow (q \land r) \), so the implication holds trivially.

Thus, the correct equivalence is proven.

### Final Answer

The original statement to prove is incorrect. The correct equivalence is:

$$ p \rightarrow (q \land r) \equiv (\neg q \lor \neg r) \rightarrow \neg p $$

This can be proven using resolution by showing that each side implies the other, as demonstrated above. The original statement with \( \land \) instead of \( \lor \) does not hold, as evidenced by the truth tables showing differing truth values in certain cases.

--- 

The rendered LaTeX is now properly formatted with mathematical expressions and logical symbols displayed correctly.