# Logic

- true and false

## Definition 

## Truth values

if I have statements p,q,r,s. Draw the truth tables of these statments
$$p: 2^4 , q:2^3,r:2^2,s:2^1$$

| p   | q   | r   | s   |     |
| --- | --- | --- | --- | --- |
| 1   | 1   | 1   | 1   |     |
| 1   | 0   | 1   | 1   |     |
| 1   | 1   | 0   | 1   |     |
| 1   | 1   | 1   | 0   |     |
| 1   | 0   | 0   | 1   |     |
| 1   | 1   | 0   | 0   |     |
| 1   | 0   | 1   | 0   |     |
| 1   | 0   | 0   | 0   |     |
| 0   | 0   | 0   | 0   |     |
| 0   | 1   | 0   | 0   |     |
| 0   | 0   | 1   | 0   |     |
| 0   | 0   | 0   | 1   |     |
| 0   | 1   | 1   | 0   |     |
| 0   | 0   | 1   | 1   |     |
| 0   | 1   | 0   | 1   |     |
| 0   | 1   | 1   | 1   |     |

## table
| $p$ | $q$ | $r$ | $s$ | $\neg{p}$ | $\neg{q}$ | $\neg{r}$ | $\neg{s}$ |
| --- | --- | --- | --- | --------- | --------- | --------- | --------- |
| 1   | 1   | 1   | 1   | 0         | 0         | 0         | 0         |
| 1   | 1   | 1   | 0   | 0         | 0         | 0         | 1         |
| 1   | 1   | 0   | 1   | 0         | 0         | 1         | 0         |
| 1   | 1   | 0   | 0   | 0         | 0         | 1         | 1         |
| 1   | 0   | 1   | 1   | 0         | 1         | 0         | 0         |
| 1   | 0   | 1   | 0   | 0         | 1         | 0         | 1         |
| 1   | 0   | 0   | 1   | 0         | 1         | 1         | 0         |
| 1   | 0   | 0   | 0   | 0         | 1         | 1         | 1         |
| 0   | 1   | 1   | 1   | 1         | 0         | 0         | 0         |
| 0   | 1   | 1   | 0   | 1         | 0         | 0         | 1         |
| 0   | 1   | 0   | 1   | 1         | 0         | 1         | 0         |
| 0   | 1   | 0   | 0   | 1         | 0         | 1         | 1         |
| 0   | 0   | 1   | 1   | 1         | 1         | 0         | 0         |
| 0   | 0   | 1   | 0   | 1         | 1         | 0         | 1         |
| 0   | 0   | 0   | 1   | 1         | 1         | 1         | 0         |
| 0   | 0   | 0   | 1   | 1         | 1         | 1         | 1         |
## Conjuction or connectivity
## Negation: $$\neg{p}$$
	if P is true then not P is false


| p   | $\neg{p}$ |
| --- | --------- |
| 1   | 0         |
| 0   | 1         |

### Or:  $$p\lor{q}$$
	Or: If at least one is true then the proposition is true

| p   | q   | $p\lor{q}$ |
| --- | --- | ---------- |
| 1   | 1   | 1          |
| 1   | 0   | 1          |
| 0   | 1   | 1          |
| 0   | 0   | 0          |
### And: $$p\land{q}$$
	And: Both of the propositions must be true

| p   | q   | $p\land{q}$ |
| --- | --- | ----------- |
| 1   | 1   | 1           |
| 1   | 0   | 0           |
| 0   | 1   | 0           |
| 0   | 0   | 0           |

### Implication: $$p\rightarrow{q}$$
if it is raining then the ground is wet
p: it is raining
q: the ground is wet

| p   | q   | $p\rightarrow{q}$ |
| --- | --- | ----------------- |
| 1   | 1   | 1                 |
| 1   | 0   | 0                 |
| 0   | 1   | 1                 |
| 0   | 0   | 1                 |

### If and only if, NXOR $$p\Leftrightarrow{q}$$

| p   | q   | $p\Leftrightarrow{q}$ |
| --- | --- | --------------------- |
| 1   | 1   | 1                     |
| 1   | 0   | 0                     |
| 0   | 1   | 0                     |
| 0   | 0   | 1                     |


## Type of proofs


### Direct proof: 

if n is an even number, so n^2 is even

p: n is even
q: n^2 is even

we have $n=2k, k\in \mathbb{Z}$
$n^2 = (2k)^2=4k^2=2*2k^2,\text{Let } m=2k^2\in \mathbb{Z}$ 
is even

therefore $p\rightarrow{q}$

### Contrapositive

$$\neg{q}\rightarrow{\neg{p}}$$
if n^2 is even, so n is even

p: $n^2$ is even
q: n is even

$\neg{q}: \text{n is odd}$
$\neg{p}: n^2\text{ is odd}$

we have $n = 2k+1, k\in{\mathbb{Z}}$
therefore n is odd

$n^2=4k^2+4k+1$
$n^2=2(2k^2+2k)+1$
therfore n^2 is odd 

if n is odd then n^2 is odd
then by contrapositive n^2 is even then n is even

### Contracdiction
$$[\neg{p}\rightarrow{C}]\rightarrow{p}$$

| p   | C   | $\neg p$ | $\neg{p}\rightarrow{C}$ | $[\neg{p}\rightarrow{C}]\rightarrow{p}$ |
| --- | --- | -------- | ----------------------- | --------------------------------------- |
| T   | F   | F        | T                       | T                                       |
| F   | F   | T        | F                       | T                                       |

If r is a real number such that $r^2=2$, then r is an irrational number.

r is a real number such that $r^2=2$ then r is a rational number.

Since r is a rational number there exists m,n such that 
$r=\frac{m}{n}$ and and m and n have no common factor greater than 1.
since $r^2=2$

$2=\frac{m^2}{n^2}$
$2n^2=m^2$
$m^2\text{ Implies } m^2 \text{ is even and m is even}$
there exists an integer p such that $m=2p$

$(2p)^2=2n^2$
$4p^2=2n^2$

we have n^2 is even -> n is an even integer. since both m and n is even 2 is a common factor of m and n which contradicts that m and n is a co prime number.

Consequently, the statement of the theorem cannot be false, and we have proved that if r is a real number such that $r^2=2$, then r is an irrational number.
## Truth table practice

1. $(p\lor{\neg{q}})\Leftrightarrow(q\rightarrow{\neg{p}})$ 

| p   | $\neg{q}$ | q   | $\neg{p}$ | $p\lor{\neg{q}}$ | $q\rightarrow{\neg{p}}$ | $(p\lor{\neg{q}})\Leftrightarrow(q\rightarrow{\neg{p}})$ |
| --- | --------- | --- | --------- | ---------------- | ----------------------- | -------------------------------------------------------- |
| 1   | 0         | 1   | 0         | 1                | 0                       | 0                                                        |
| 1   | 1         | 0   | 0         | 1                | 1                       | 1                                                        |
| 0   | 0         | 1   | 1         | 0                | 1                       | 0                                                        |
| 0   | 1         | 0   | 1         | 1                | 1                       | 1                                                        |


2. $[p\land{(\neg{q}\rightarrow{p})}]\land\neg[(p\Leftrightarrow{\neg{q}})\rightarrow(q\lor{\neg{p}})]$


| p   | q   | $\neg{p}$ | $\neg{q}$ | $(\neg{q}\rightarrow{p})$ | $p\Leftrightarrow{\neg{q}}$ | $q\lor{\neg{p}}$ | $(p\Leftrightarrow{\neg{q}})\rightarrow(q\lor{\neg{p}})$ | $\neg[(p\Leftrightarrow{\neg{q}})\rightarrow(q\lor{\neg{p}})]$ | $[p\land{(\neg{q}\rightarrow{p})}]$ | $[p\land{(\neg{q}\rightarrow{p})}]\land\neg[(p\Leftrightarrow{\neg{q}})\rightarrow(q\lor{\neg{p}})]$ |
| --- | --- | --------- | --------- | ------------------------- | --------------------------- | ---------------- | -------------------------------------------------------- | -------------------------------------------------------------- | ----------------------------------- | ---------------------------------------------------------------------------------------------------- |
| 1   | 1   | 0         | 0         | 1                         | 0                           | 1                | 1                                                        | 0                                                              | 1                                   | 0                                                                                                    |
| 1   | 0   | 0         | 1         | 1                         | 1                           | 0                | 0                                                        | 1                                                              | 1                                   | 1                                                                                                    |
| 0   | 1   | 1         | 0         | 1                         | 1                           | 1                | 1                                                        | 0                                                              | 0                                   | 0                                                                                                    |
| 0   | 0   | 1         | 1         | 0                         | 0                           | 1                | 1                                                        | 0                                                              | 0                                   | 0                                                                                                    |

3. $[q\Leftrightarrow{(r\rightarrow \neg{p})}]\lor[(\neg{q}\rightarrow{p})\Leftrightarrow{r}]$


| p   | q   | r   | $\neg{p}$ | $\neg{q}$ | $(r\rightarrow \neg{p})$ | $[q\Leftrightarrow{(r rightarrow \neg{p})}]$ | $(\neg{q}\rightarrow{p})$ | $[(\neg{q}\rightarrow{p})\Leftrightarrow{r}]$ | $[q\Leftrightarrow{(r\rightarrow \neg{p})}]\lor[(\neg{q}\rightarrow{p})\Leftrightarrow{r}]$ |
| --- | --- | --- | --------- | --------- | ------------------------ | -------------------------------------------- | ------------------------- | --------------------------------------------- | ------------------------------------------------------------------------------------------- |
| 1   | 1   | 1   | 0         | 0         | 0                        | 0                                            | 1                         | 1                                             | 1                                                                                           |
| 1   | 1   | 0   | 0         | 0         | 1                        | 1                                            | 1                         | 0                                             | 1                                                                                           |
| 1   | 0   | 1   | 0         | 1         | 0                        | 1                                            | 1                         | 0                                             | 1                                                                                           |
| 1   | 0   | 0   | 0         | 1         | 1                        | 0                                            | 1                         | 0                                             | 0                                                                                           |
| 0   | 1   | 1   | 1         | 0         | 1                        | 1                                            | 1                         | 1                                             | 1                                                                                           |
| 0   | 1   | 0   | 1         | 0         | 0                        | 0                                            | 1                         | 1                                             | 1                                                                                           |
| 0   | 0   | 1   | 1         | 1         | 1                        | 0                                            | 0                         | 1                                             | 0                                                                                           |
| 0   | 0   | 0   | 1         | 1         | 0                        | 1                                            | 0                         | 1                                             | 1                                                                                           |


4. $(p\Leftrightarrow\neg{q})\Leftrightarrow(q\rightarrow{p})$

| p   | q   | $\neg{p}$ | $\neg{q}$ | $(p\Leftrightarrow\neg{q})$ | $q\rightarrow{p}$ | $(p\Leftrightarrow\neg{q})\Leftrightarrow(q\rightarrow{p})$ |
| --- | --- | --------- | --------- | --------------------------- | ----------------- | ----------------------------------------------------------- |
| 1   | 1   | 0         | 0         | 0                           | 1                 | 0                                                           |
| 1   | 0   | 0         | 1         | 1                           | 1                 | 1                                                           |
| 0   | 1   | 1         | 0         | 1                           | 0                 | 0                                                           |
| 0   | 0   | 1         | 1         | 0                           | 1                 | 0                                                           |


### $\text{ Proof }\sqrt{7}\text{ is irrational}$

$7=\frac{a^2}{b^2};a,b\in \mathbb{Z}$
a,b are co primes

$7b^2=a^2$
Since $7b^2=a^2, a^2\text{ is a multiple of 7}$
so a is divisible by 7 (since 7 is a prime number)
$a=7k$



